Finished base theorems, added circuit definition and a couple of lemmas

src/matroid.lean
@@ -31,87 +31,10 @@ def base (m : matroid X) (A : finset X) := m.ind A ∧ ∀ x ∉ A, ¬m.ind (ins
 
 @[simp] lemma base_ind {A : finset X} : m.base A → m.ind A := λ x, x.1
 
-lemma base_eq_card {A B : finset X} (hA : m.base A) (hB : m.base B) : A.card = B.card := 
-begin
-  by_contradiction,
-  wlog : A.card ≤ B.card := le_total A.card B.card using [A B, B A],
-  replace h := nat.lt_of_le_and_ne case h,
-  rcases m.ind_exchange _ _ (base_ind hA) (base_ind hB) h with ⟨w, wB, wA, winsert⟩,
-  exact hA.2 w wA winsert,
-end
+def circuit (m : matroid X) (C : finset X) := ¬ m.ind C ∧ ∀ x ∈ C, m.ind (C.erase x)
 
-theorem base_exists : ∃ A, m.base A :=
-begin
-  by_contradiction,
-  push_neg at h,
-  suffices ind_unbounded : ∀ k, ∃ A, (m.ind A) ∧ A.card = k, {
-    rcases ind_unbounded (fintype.card X + 1) with ⟨A, Aind, Acard⟩,
-    have Acard_le := finset.card_le_univ A,
-    linarith,
-  },
-  intro k,
-  induction k, {
-    use ∅,
-    simp only [finset.card_empty, ind_empty, eq_self_iff_true, and_self],
-  }, {
-    rcases k_ih with ⟨A, Aind, Acard⟩,
-    specialize h A,    
-    rw base at h,
-    push_neg at h,
-    rcases h Aind with ⟨x, xA, ind_insert⟩,
-    use [insert x A, ind_insert],
-    rw ← Acard,
-    exact finset.card_insert_of_not_mem xA,
-  }
-end
+@[simp] lemma circuit_not_ind {C : finset X} : m.circuit C → ¬ m.ind C := λ x, x.1
 
-theorem base_not_subset {A B} : m.base A → m.base B → A ⊆ B → A = B :=
-begin
-  rintro Abase Bbase h_subset,
-  exact finset.eq_of_card_eq_subset h_subset (base_eq_card Abase Bbase),
-end
 
--- TODO: use in base_exists
-lemma ind_extension {A} : m.ind A → ∃ B, A ⊆ B ∧ m.base B :=
-begin
-  sorry,
-end
-
-lemma base_iff_ind_and_eq_card_base {A B} (Abase : m.base A) : (m.ind B ∧ A.card = B.card) ↔ m.base B :=
-begin
-  split, {
-    rintro ⟨Bind, Acard⟩,
-    use Bind,
-    intros x xB h_insert_ind,
-    sorry,
-  }, {
-    intro Bbase,
-    exact ⟨Bbase.1, base_eq_card Abase Bbase⟩,
-  }
-end
-
-theorem base_exchange {A B} : m.base A → m.base B → A ≠ B → ∀ x ∈ A \ B, ∃ b ∈ B, b ∉ A ∧ m.base (insert b (A.erase x)) :=
-begin
-  intros Abase Bbase h_neq x xA,
-  rcases m.ind_exchange (A.erase x) B _ Bbase.1 _ with ⟨c, cB, cA, cinsert⟩,
-  use [c, cB],
-  {
-    rw [mem_erase] at cA,
-    push_neg at cA,
-    rw mem_sdiff at xA,
-    split, {
-      finish,
-    }, {
-      apply (base_iff_ind_and_eq_card_base Abase).1,
-      use cinsert,
-      sorry,
-    },
-  }, { 
-    exact m.ind_subset _ _ (erase_subset _ _) Abase.1, 
-  }, {
-    rw [← base_eq_card Abase Bbase, card_erase_of_mem xA],
-    exact nat.pred_lt (card_ne_zero_of_mem xA),
-  },
-end
 
 end matroid
