src/base.lean
@@ -1,0 +1,99 @@
+import data.fintype.basic
+import tactic
+import matroid
+import finset
+
+variables {X : Type*} [fintype X] [decidable_eq X] {m : matroid X}
+
+open finset
+
+namespace matroid
+
+lemma base_eq_card {A B : finset X} (hA : m.base A) (hB : m.base B) : A.card = B.card := 
+begin
+  by_contradiction,
+  wlog : A.card ≤ B.card := le_total A.card B.card using [A B, B A],
+  replace h := nat.lt_of_le_and_ne case h,
+  rcases m.ind_exchange _ _ (base_ind hA) (base_ind hB) h with ⟨w, wB, wA, winsert⟩,
+  exact hA.2 w wA winsert,
+end
+
+lemma ind_subset_base {A} : m.ind A → ∃ B, A ⊆ B ∧ m.base B :=
+begin
+  intro Aind,
+  by_contradiction,
+  push_neg at h,
+  suffices ind_unbounded : ∀ k ≥ A.card, ∃ B, A ⊆ B ∧ (m.ind B) ∧ B.card = k, {
+    rcases ind_unbounded (fintype.card X + 1) _ with ⟨B, h_suibset, Bind, Bcard⟩,
+    have Bcard_le := card_le_univ B,
+    linarith,
+    have Acard_le := card_le_univ A,
+    linarith,
+  },
+  apply nat.le_induction, {
+    use [A, subset.refl A, Aind, rfl],
+  }, {
+    rintro n Acard ⟨B, h_subset, Bind, Bcard⟩,
+    specialize h B h_subset,
+    rw base at h,
+    push_neg at h,
+    rcases h Bind with ⟨x, xB, x_insert⟩,
+    use [insert x B],
+    rw ← Bcard,
+    use [subset.trans h_subset (subset_insert _ _), x_insert, card_insert_of_not_mem xB],
+  }
+end
+
+theorem base_exists : ∃ A, m.base A :=
+begin
+  obtain ⟨B, _, Bbase⟩ := ind_subset_base m.ind_empty,
+  exact ⟨B, Bbase⟩,
+end
+
+theorem base_not_subset {A B} : m.base A → m.base B → A ⊆ B → A = B :=
+begin
+  rintro Abase Bbase h_subset,
+  exact finset.eq_of_subset_card_eq_card h_subset (base_eq_card Abase Bbase),
+end
+
+lemma ind_and_card_eq_card_base_iff_base {A B} (Abase : m.base A) : (m.ind B ∧ A.card = B.card) ↔ m.base B :=
+begin
+  split, {
+    rintro ⟨Bind, Acard⟩,
+    use Bind,
+    intros x xB h_insert_ind,
+    obtain ⟨C, Bsubset, Cbase⟩ := ind_subset_base h_insert_ind,
+    replace Bsubset := card_le_of_subset Bsubset,
+    rw [base_eq_card Abase Cbase] at Acard,
+    rw card_insert_of_not_mem xB at Bsubset,
+    linarith,
+  }, {
+    intro Bbase,
+    exact ⟨Bbase.1, base_eq_card Abase Bbase⟩,
+  }
+end
+
+theorem base_exchange {A B} : m.base A → m.base B → A ≠ B → ∀ x ∈ A \ B, ∃ b ∈ B, b ∉ A ∧ m.base (insert b (A.erase x)) :=
+begin
+  intros Abase Bbase h_neq x xA,
+  rcases m.ind_exchange (A.erase x) B _ Bbase.1 _ with ⟨c, cB, cA, cinsert⟩,
+  use [c, cB],
+  {
+    rw mem_sdiff at xA,
+    split, {
+      finish,
+    }, {
+      apply (ind_and_card_eq_card_base_iff_base Abase).1,
+      use cinsert,
+      rw [card_insert_of_not_mem cA, card_erase_of_mem' xA.1],
+    },
+  }, { 
+    exact m.ind_subset _ _ (erase_subset _ _) Abase.1, 
+  }, {
+    rw mem_sdiff at xA,
+    rw [← base_eq_card Abase Bbase, card_erase_of_mem xA.1],
+    exact nat.pred_lt (card_ne_zero_of_mem xA.1),
+  },
+end
+
+end matroid
