src/circuit.lean
@@ -1,0 +1,34 @@
+import data.fintype.basic
+import tactic
+import matroid
+import finset
+
+variables {X : Type*} [fintype X] [decidable_eq X] {m : matroid X}
+
+open finset
+
+namespace matroid
+
+lemma circuit_sdiff {A B} : m.circuit A → B ⊆ A → B ≠ ∅ → m.ind (A \ B) :=
+begin
+  rintro ⟨Anind, Aerase⟩ Bsubset Bnonempty, 
+  rw ← nonempty_iff_ne_empty at Bnonempty,
+  rcases Bnonempty with ⟨x, xB⟩,
+  have xA := Bsubset xB,
+  refine m.ind_subset _ (A.erase x) _ (Aerase x xA),
+  exact sdiff_subset_erase_of_mem xB,
+end 
+
+lemma circuit_subset {A B} : m.circuit A → B ⊂ A → m.ind B :=
+begin 
+  rintro ⟨Anind, Aerase⟩ Bsubset,
+  rw ssubset_iff at Bsubset,
+  rcases Bsubset with ⟨x, xB, x_insert⟩,
+  rw insert_subset at x_insert,
+  cases x_insert with xA h_subset,  
+  apply m.ind_subset _ (A.erase x) _ (Aerase x xA),
+  rw ← erase_eq_of_not_mem xB,
+  exact erase_subset_erase x h_subset,
+end 
+
+end matroid
