src/finset.lean
@@ -3,17 +3,47 @@ import tactic
 
 variables {X : Type*} [fintype X] [decidable_eq X]
 
-lemma finset.eq_of_card_eq_subset {A B : finset X} : A ⊆ B → A.card = B.card → A = B :=
+namespace finset
+
+open finset
+
+lemma card_erase_of_mem' {A : finset X} {x} (h : x ∈ A) : (A.erase x).card + 1 = A.card :=
+begin
+  rw [card_erase_of_mem h, nat.add_one, nat.succ_pred_eq_of_pos],
+  rw [gt_iff_lt, pos_iff_ne_zero],
+  exact card_ne_zero_of_mem h,
+end
+
+lemma eq_of_subset_card_eq_card {A B : finset X} : A ⊆ B → A.card = B.card → A = B :=
 begin
   intros h_subset h_card,
   induction B using finset.induction_on generalizing A, {
-    simpa only [finset.card_empty, finset.card_eq_zero] using h_card,
+    simpa only [card_empty, card_eq_zero] using h_card,
   },
   case h₂ : x B x_mem ih {
-    specialize @ih (A \ {x}),
+    rw subset_insert_iff at h_subset,
+    rw card_insert_of_not_mem x_mem at h_card,
     have t : x ∈ A, from by {
-      sorry,
+      by_contradiction,
+      replace h_subset := card_le_of_subset h_subset,
+      rw [erase_eq_of_not_mem h, h_card] at h_subset,
+      simpa only [add_le_iff_nonpos_right, nonpos_iff_eq_zero] using h_subset,
     },
-    sorry,
+    rw [← card_erase_of_mem' t, add_left_inj] at h_card,
+    specialize ih h_subset h_card,
+    apply_fun insert x at ih,
+    rwa insert_erase t at ih,
   },
 end
+
+example {A : finset X} {x} : A.erase x = A \ {x} := (sdiff_singleton_eq_erase x A).symm
+
+lemma sdiff_subset_erase_of_mem {A B : finset X} {x} : x ∈ B → A \ B ⊆ A.erase x :=
+begin
+  intros xB,
+  rw [← sdiff_singleton_eq_erase x A],
+  apply sdiff_subset_sdiff (subset.refl _) _,
+  rwa singleton_subset_iff,
+end
+
+end finset
